code/verification/Entails.v
@@ -1,0 +1,26 @@
+From Stdlib Require Import List.
+Import ListNotations.
+From RocqSAT Require Import Lit CNF Evaluation WellFormed Trans.
+
+Inductive Entails: CNF -> PA -> Prop :=
+| e_intro (f: CNF) (n: PA):
+  (forall (m: PA), 
+    f_eval m f = Some true -> m_eval m n = Some true) ->
+  NoDecisions n ->
+  Entails f n
+| e_step (f: CNF) (m n: PA) (l: Lit):
+  (forall (m': PA), 
+    f_eval m' f = Some true /\
+    m_eval m' m = Some true /\
+    l_eval m' l = Some true -> m_eval m' n = Some true) ->
+  NoDecisions n ->
+  Entails f m ->
+  Entails f (m ++d l ++a n).
+
+Lemma trans_entails: forall (m m': PA) (f: CNF) (Hwf: WellFormed m f) (Hwf': WellFormed m' f),
+  state m f Hwf ==> state m' f Hwf' -> Entails f m -> Entails f m'.
+Admitted.
+
+Lemma derivation_entails: forall (m m': PA) (f: CNF) (Hwf: WellFormed m f) (Hwf': WellFormed m' f),
+  state m f Hwf ==>* state m' f Hwf' -> Entails f m -> Entails f m'.
+Admitted.
